
$$\Large
\begin{array}{l}
\exists a_{n}=\{a_{1}, a_{2},\dots a_{n}\}\\
A=\sum\limits\limits_{i=1}^{n}{a_{i}}=a_{1}+a_{2}+\dots+a_{n}\\
B=\prod\limits\limits_{i=1}^{n}{a_{i}}=a_{1}\cdot a_{2}\cdot \dots \cdot a_{n}\\
a_{k}^{\ast}=\prod\limits_{i=1}^{k-1}{a_{i}}\cdot\prod\limits_{i=k+1}^{n}{a_{i}}=\dfrac{B}{a_{k}}\\
C=\sum\limits_{i=1}^{n}{a_{i}^{\ast}}=\sum\limits_{i=1}^{n}{\dfrac{B}{a_{i}}}=B\cdot E\\
D=\prod\limits_{i=1}^{n}{a_{i}^{\ast}}=\prod\limits_{i=1}^{n}{\dfrac{B}{a_{i}}}=\dfrac{B^{n}}{B}=B^{n-1}\\
E=\sum\limits_{i=1}^{n}{a_{i}^{-1}}=\sum\limits_{i=1}^{n}{\dfrac{1}{a_{i}}}=\\
=\dfrac{1}{a_{1}}+\dfrac{1}{a_{2}}+\dfrac{1}{a_{3}}+\dots\dfrac{1}{a_{n}}=\\
=\dfrac{a_{2}a_{3}\dots a_{n}+a_{1}a_{3}\dots a_{n}+\dots}{a_{1}a_{2}a_{3}\dots a_{n}}=\\
\dfrac{a_{1}^{\ast}+a_{2}^{\ast}+\dots+a_{n}^{\ast}}{B}=\dfrac{C}{B}
\end{array}
$$

